

2022-2023

2-2

A

$$1 \qquad 2x_1^2+ax_2^2+2x_3^2+2x_1x_2+2x_1x_3+2x_2x_3=3$$
$$y_1^2+y_2^2+by_3^2=3 \qquad a;b \qquad T$$

$$\begin{array}{ccc} \text{O} & 1 & \text{O} & 1 \\ \text{B}^{x_1} & & \text{B}^{y_1} & \\ @_{x_2} & \text{C} & @_{y_2} & \text{C} \\ & & x_3 & y_3 \end{array} = T$$

$$2 \quad \mathbb{P} \qquad \mathbb{P}^{2-2}$$
$$V_1 = \left(\begin{array}{cc} x & x \\ y & z \end{array} \right) \begin{array}{c} ! \\ x;y;z \in \mathbb{P} \end{array}; V_2 = \left(\begin{array}{cc} a & b \\ a & c \end{array} \right) \begin{array}{c} ! \\ a;b;c \in \mathbb{P} \end{array}$$

$$1 \qquad V_1;V_2 \qquad \mathbb{P}^{2-2}$$
$$2 \qquad V_1+V_2 \qquad V_1 \setminus V_2$$

$$3 \qquad \begin{array}{ccc} \text{O} & & 1 \\ 1 & 1 & 0 \\ \text{B} & & \text{C} \\ @ & 1 & 3 & 0 \\ & 1 & 0 & 2 \end{array} A = \begin{array}{c} \text{C} \\ \text{A} \end{array}$$

A Jordan

$$4 \qquad \frac{x-1}{1} = \frac{y}{3} = \frac{z}{3} \qquad z$$

$$5 \qquad \mathbb{P} \qquad V \qquad ^2 =$$
$$1 \qquad V = (V) \qquad ^1(0)$$
$$2 \qquad V \qquad (V); \qquad ^1(0)$$

$$6 \qquad \frac{x^2}{a^2} + \frac{y^2}{b^2} - \frac{z^2}{c^2} = 1$$

$$7 \quad A \quad n \qquad B \quad n \qquad jA+Bj \quad -jAj+jBj \qquad B=0$$

A